James C - renamed “safe -> normal”, “normal -> ‘”

isabelle/Chapter20_1_Language.thy
@@ -22,15 +22,15 @@ where "is_valid_type tyvars (Arr t1 t2) = (is_valid_type tyvars t1 & is_valid_ty
     | "is_valid_type tyvars (Rec t) = (is_valid_type (expand_set tyvars) t)"
     | "is_valid_type tyvars (All t) = (is_valid_type (expand_set tyvars) t)"
 
-primrec free_type_vars :: "type => nat set"
-where "free_type_vars (Tyvar v) = {v}"
-    | "free_type_vars (Arr e1 e2) = free_type_vars e1 Un free_type_vars e2"
-    | "free_type_vars Unit = {}"
-    | "free_type_vars (Prod e1 e2) = free_type_vars e1 Un free_type_vars e2"
-    | "free_type_vars Void = {}"
-    | "free_type_vars (Sum e1 e2) = free_type_vars e1 Un free_type_vars e2"
-    | "free_type_vars (Rec t) = redr_set (free_type_vars t)"
-    | "free_type_vars (All t) = redr_set (free_type_vars t)"
+primrec type_free_vars :: "type => nat set"
+where "type_free_vars (Tyvar v) = {v}"
+    | "type_free_vars (Arr e1 e2) = type_free_vars e1 Un type_free_vars e2"
+    | "type_free_vars Unit = {}"
+    | "type_free_vars (Prod e1 e2) = type_free_vars e1 Un type_free_vars e2"
+    | "type_free_vars Void = {}"
+    | "type_free_vars (Sum e1 e2) = type_free_vars e1 Un type_free_vars e2"
+    | "type_free_vars (Rec t) = redr_set (type_free_vars t)"
+    | "type_free_vars (All t) = redr_set (type_free_vars t)"
 
 primrec type_sub_from :: "nat => type => type"
 where "type_sub_from n (Tyvar v) = Tyvar (subr n v)"
@@ -52,20 +52,20 @@ where "type_incr_from n (Tyvar v) = Tyvar (incr n v)"
     | "type_incr_from n (Rec t) = Rec (type_incr_from (Suc n) t)"
     | "type_incr_from n (All t) = All (type_incr_from (Suc n) t)"
 
-primrec type_subst :: "type => type => nat => type"
-where "type_subst (Tyvar v) t x = (if v = x then t else Tyvar v)"
-    | "type_subst (Arr t1 t2) t x = Arr (type_subst t1 t x) (type_subst t2 t x)"
-    | "type_subst Unit t x = Unit"
-    | "type_subst (Prod t1 t2) t x = Prod (type_subst t1 t x) (type_subst t2 t x)"
-    | "type_subst Void t x = Void"
-    | "type_subst (Sum t1 t2) t x = Sum (type_subst t1 t x) (type_subst t2 t x)"
-    | "type_subst (Rec t0) t x = Rec (type_subst t0 (type_incr_from 0 t) (Suc x))"
-    | "type_subst (All t0) t x = All (type_subst t0 (type_incr_from 0 t) (Suc x))"
+primrec type_subst' :: "type => type => nat => type"
+where "type_subst' (Tyvar v) t x = (if v = x then t else Tyvar v)"
+    | "type_subst' (Arr t1 t2) t x = Arr (type_subst' t1 t x) (type_subst' t2 t x)"
+    | "type_subst' Unit t x = Unit"
+    | "type_subst' (Prod t1 t2) t x = Prod (type_subst' t1 t x) (type_subst' t2 t x)"
+    | "type_subst' Void t x = Void"
+    | "type_subst' (Sum t1 t2) t x = Sum (type_subst' t1 t x) (type_subst' t2 t x)"
+    | "type_subst' (Rec t0) t x = Rec (type_subst' t0 (type_incr_from 0 t) (Suc x))"
+    | "type_subst' (All t0) t x = All (type_subst' t0 (type_incr_from 0 t) (Suc x))"
 
-definition safe_type_subst :: "type => type => type"
-where "safe_type_subst e e' = type_sub_from 0 (type_subst e (type_incr_from 0 e') 0)"
+definition type_subst :: "type => type => type"
+where "type_subst e e' = type_sub_from 0 (type_subst' e (type_incr_from 0 e') 0)"
 
-lemma [simp]: "free_type_vars (type_incr_from n e) = incr n ` free_type_vars e"
+lemma [simp]: "type_free_vars (type_incr_from n e) = incr n ` type_free_vars e"
 by (induction e arbitrary: n, auto)
 
 lemma valid_incr_type: "is_valid_type (expand_set_at m s) (type_incr_from m t) = is_valid_type s t"
@@ -84,17 +84,17 @@ by (induction t arbitrary: n m, simp_all)
 lemma [simp]: "m <= n ==> type_incr_from m (type_incr_from n t) = type_incr_from (Suc n) (type_incr_from m t)"
 by (induction t arbitrary: n m, simp_all)
 
-lemma [simp]: "type_incr_from m (type_subst a t x) = type_subst (type_incr_from m a) (type_incr_from m t) (incr m x)"
+lemma [simp]: "type_incr_from m (type_subst' a t x) = type_subst' (type_incr_from m a) (type_incr_from m t) (incr m x)"
 by (induction a arbitrary: t x m, auto simp add: incr_def)
 
 primrec type_incr_by :: "nat => type => type"
 where "type_incr_by 0 e = e"
     | "type_incr_by (Suc n) e = type_incr_from 0 (type_incr_by n e)"
 
-lemma [simp]:  "redr_set_by n (free_type_vars (type_incr_by n e)) = free_type_vars e" 
+lemma [simp]:  "redr_set_by n (type_free_vars (type_incr_by n e)) = type_free_vars e" 
 by (induction n, simp_all) 
 
-lemma [simp]: "free_type_vars (type_subst e e' x) = (if x : free_type_vars e then free_type_vars e - {x} Un free_type_vars e' else free_type_vars e)"
+lemma [simp]: "type_free_vars (type_subst' e e' x) = (if x : type_free_vars e then type_free_vars e - {x} Un type_free_vars e' else type_free_vars e)"
 by (induction e arbitrary: e' x, auto)
 
 datatype expr = 
@@ -169,26 +169,26 @@ where "sub_from n (Var v) = Var (if v < n then v else v - 1)"
     | "sub_from n (TyLam e) = TyLam (sub_from n e)"
     | "sub_from n (TyAp t e) = TyAp t (sub_from n e)"
 
-primrec subst :: "expr => expr => nat => expr"
-where "subst (Var v) e x = (if v = x then e else Var v)"
-    | "subst (Lam t b) e x = Lam t (subst b (incr_from 0 e) (Suc x))"
-    | "subst (Ap e1 e2) e x = Ap (subst e1 e x) (subst e2 e x)"
-    | "subst (Fix t b) e x = Fix t (subst b (incr_from 0 e) (Suc x))"
-    | "subst Triv e x = Triv"
-    | "subst (Pair e1 e2) e x = Pair (subst e1 e x) (subst e2 e x)"
-    | "subst (ProjL n) e x = ProjL (subst n e x)"
-    | "subst (ProjR n) e x = ProjR (subst n e x)"
-    | "subst (Abort t n) e x = Abort t (subst n e x)"
-    | "subst (InL t t' n) e x = InL t t' (subst n e x)"
-    | "subst (InR t t' n) e x = InR t t' (subst n e x)"
-    | "subst (Case n el er) e x = Case (subst n e x) (subst el (incr_from 0 e) (Suc x)) (subst er (incr_from 0 e) (Suc x))"
-    | "subst (Fold t n) e x = Fold t (subst n e x)"
-    | "subst (Unfold n) e x = Unfold (subst n e x)"
-    | "subst (TyLam n) e x = TyLam (subst n e x)"
-    | "subst (TyAp t n) e x = TyAp t (subst n e x)"
+primrec subst' :: "expr => expr => nat => expr"
+where "subst' (Var v) e x = (if v = x then e else Var v)"
+    | "subst' (Lam t b) e x = Lam t (subst' b (incr_from 0 e) (Suc x))"
+    | "subst' (Ap e1 e2) e x = Ap (subst' e1 e x) (subst' e2 e x)"
+    | "subst' (Fix t b) e x = Fix t (subst' b (incr_from 0 e) (Suc x))"
+    | "subst' Triv e x = Triv"
+    | "subst' (Pair e1 e2) e x = Pair (subst' e1 e x) (subst' e2 e x)"
+    | "subst' (ProjL n) e x = ProjL (subst' n e x)"
+    | "subst' (ProjR n) e x = ProjR (subst' n e x)"
+    | "subst' (Abort t n) e x = Abort t (subst' n e x)"
+    | "subst' (InL t t' n) e x = InL t t' (subst' n e x)"
+    | "subst' (InR t t' n) e x = InR t t' (subst' n e x)"
+    | "subst' (Case n el er) e x = Case (subst' n e x) (subst' el (incr_from 0 e) (Suc x)) (subst' er (incr_from 0 e) (Suc x))"
+    | "subst' (Fold t n) e x = Fold t (subst' n e x)"
+    | "subst' (Unfold n) e x = Unfold (subst' n e x)"
+    | "subst' (TyLam n) e x = TyLam (subst' n e x)"
+    | "subst' (TyAp t n) e x = TyAp t (subst' n e x)"
 
-definition safe_subst :: "expr => expr => expr"
-where "safe_subst e e' = sub_from 0 (subst e (incr_from 0 e') 0)"
+definition subst :: "expr => expr => expr"
+where "subst e e' = sub_from 0 (subst' e (incr_from 0 e') 0)"
 
 lemma [simp]: "free_vars (incr_from n e) = incr n ` free_vars e"
 by (induction e arbitrary: n, auto)
@@ -200,7 +200,7 @@ where "incr_by 0 e = e"
 lemma [simp]:  "redr_set_by n (free_vars (incr_by n e)) = free_vars e" 
 by (induction n, simp_all) 
 
-lemma [simp]: "free_vars (subst e e' x) = (if x : free_vars e then free_vars e - {x} Un free_vars e' else free_vars e)"
+lemma [simp]: "free_vars (subst' e e' x) = (if x : free_vars e then free_vars e - {x} Un free_vars e' else free_vars e)"
 by (induction e arbitrary: e' x, auto)
 
 lemma [simp]: "m <= n ==> incr_from (Suc n) (incr_from m e) = incr_from m (incr_from n e)"
@@ -209,17 +209,17 @@ by (induction e arbitrary: m n, simp_all add: incr_def)
 lemma [simp]: "m <= n ==> n ~: free_vars e ==> sub_from (Suc n) (incr_from m e) = incr_from m (sub_from n e)"
 by (induction e arbitrary: n m, auto simp add: incr_def)
 
-lemma [simp]: "m <= x ==> subst (incr_from m e) (incr_from m e') (Suc x) = incr_from m (subst e e' x)"
+lemma [simp]: "m <= x ==> subst' (incr_from m e) (incr_from m e') (Suc x) = incr_from m (subst' e e' x)"
 proof (induction e arbitrary: m e' x) 
 case (Var v) 
   thus ?case by (simp add: incr_def)
 next case (Lam t b) 
-  hence "subst (incr_from (Suc m) b) (incr_from (Suc m) (incr_from 0 e')) (Suc (Suc x)) = incr_from (Suc m) (subst b (incr_from 0 e') (Suc x))" by blast 
+  hence "subst' (incr_from (Suc m) b) (incr_from (Suc m) (incr_from 0 e')) (Suc (Suc x)) = incr_from (Suc m) (subst' b (incr_from 0 e') (Suc x))" by blast 
   thus ?case by simp
 next case (Ap e1 e2) 
   thus ?case by simp
 next case (Fix t b) 
-  hence "subst (incr_from (Suc m) b) (incr_from (Suc m) (incr_from 0 e')) (Suc (Suc x)) = incr_from (Suc m) (subst b (incr_from 0 e') (Suc x))" by blast
+  hence "subst' (incr_from (Suc m) b) (incr_from (Suc m) (incr_from 0 e')) (Suc (Suc x)) = incr_from (Suc m) (subst' b (incr_from 0 e') (Suc x))" by blast
   thus ?case by simp
 next case Triv 
   thus ?case by simp
@@ -236,9 +236,9 @@ next case (InL t t' e)
 next case (InR t t' e) 
   thus ?case by simp
 next case (Case e el er) 
-  from Case have "subst (incr_from m e) (incr_from m e') (Suc x) = incr_from m (subst e e' x)" by blast
-  moreover from Case have "subst (incr_from (Suc m) el) (incr_from (Suc m) (incr_from 0 e')) (Suc (Suc x)) = incr_from (Suc m) (subst el (incr_from 0 e') (Suc x))" by blast
-  moreover from Case have "subst (incr_from (Suc m) er) (incr_from (Suc m) (incr_from 0 e')) (Suc (Suc x)) = incr_from (Suc m) (subst er (incr_from 0 e') (Suc x))" by (metis Suc_le_mono)
+  from Case have "subst' (incr_from m e) (incr_from m e') (Suc x) = incr_from m (subst' e e' x)" by blast
+  moreover from Case have "subst' (incr_from (Suc m) el) (incr_from (Suc m) (incr_from 0 e')) (Suc (Suc x)) = incr_from (Suc m) (subst' el (incr_from 0 e') (Suc x))" by blast
+  moreover from Case have "subst' (incr_from (Suc m) er) (incr_from (Suc m) (incr_from 0 e')) (Suc (Suc x)) = incr_from (Suc m) (subst' er (incr_from 0 e') (Suc x))" by (metis Suc_le_mono)
   ultimately show ?case by simp
 next case (Fold t e) 
   thus ?case by simp
@@ -250,29 +250,29 @@ next case (TyAp t e)
   thus ?case by simp
 qed 
 
-lemma [simp]: "sub_from n (subst (incr_from n e) e' n) = e" 
+lemma [simp]: "sub_from n (subst' (incr_from n e) e' n) = e" 
 by (induction e arbitrary: n e', simp_all add: incr_def)
 
-lemma [simp]: "safe_subst (incr_from 0 e) e' = e"
-by (simp add: safe_subst_def) 
+lemma [simp]: "subst (incr_from 0 e) e' = e"
+by (simp add: subst_def) 
 
-primrec subst_type :: "expr => type => nat => expr"
-where "subst_type (Var v) e x = Var v"
-    | "subst_type (Lam t b) e x = Lam (type_subst t e x) b"
-    | "subst_type (Ap e1 e2) e x = Ap (subst_type e1 e x) (subst_type e2 e x)"
-    | "subst_type (Fix t b) e x = Fix (type_subst t e x) (subst_type b e x)"
-    | "subst_type Triv e x = Triv"
-    | "subst_type (Pair e1 e2) e x = Pair (subst_type e1 e x) (subst_type e2 e x)"
-    | "subst_type (ProjL n) e x = ProjL (subst_type n e x)"
-    | "subst_type (ProjR n) e x = ProjR (subst_type n e x)"
-    | "subst_type (Abort t n) e x = Abort (type_subst t e x) (subst_type n e x)"
-    | "subst_type (InL t t' n) e x = InL (type_subst t e x) (type_subst t' e x) (subst_type n e x)"
-    | "subst_type (InR t t' n) e x = InR (type_subst t e x) (type_subst t' e x) (subst_type n e x)"
-    | "subst_type (Case n el er) e x = Case (subst_type n e x) (subst_type el e x) (subst_type er e x)"
-    | "subst_type (Fold t n) e x = Fold (type_subst t e x) (subst_type n e x)"
-    | "subst_type (Unfold n) e x = Unfold (subst_type n e x)"
-    | "subst_type (TyLam n) e x = TyLam (subst_type n e (Suc x))"
-    | "subst_type (TyAp t n) e x = TyAp (type_subst t e x) (subst_type n e x)"
+primrec subst_type' :: "expr => type => nat => expr"
+where "subst_type' (Var v) e x = Var v"
+    | "subst_type' (Lam t b) e x = Lam (type_subst' t e x) b"
+    | "subst_type' (Ap e1 e2) e x = Ap (subst_type' e1 e x) (subst_type' e2 e x)"
+    | "subst_type' (Fix t b) e x = Fix (type_subst' t e x) (subst_type' b e x)"
+    | "subst_type' Triv e x = Triv"
+    | "subst_type' (Pair e1 e2) e x = Pair (subst_type' e1 e x) (subst_type' e2 e x)"
+    | "subst_type' (ProjL n) e x = ProjL (subst_type' n e x)"
+    | "subst_type' (ProjR n) e x = ProjR (subst_type' n e x)"
+    | "subst_type' (Abort t n) e x = Abort (type_subst' t e x) (subst_type' n e x)"
+    | "subst_type' (InL t t' n) e x = InL (type_subst' t e x) (type_subst' t' e x) (subst_type' n e x)"
+    | "subst_type' (InR t t' n) e x = InR (type_subst' t e x) (type_subst' t' e x) (subst_type' n e x)"
+    | "subst_type' (Case n el er) e x = Case (subst_type' n e x) (subst_type' el e x) (subst_type' er e x)"
+    | "subst_type' (Fold t n) e x = Fold (type_subst' t e x) (subst_type' n e x)"
+    | "subst_type' (Unfold n) e x = Unfold (subst_type' n e x)"
+    | "subst_type' (TyLam n) e x = TyLam (subst_type' n e (Suc x))"
+    | "subst_type' (TyAp t n) e x = TyAp (type_subst' t e x) (subst_type' n e x)"
 
 primrec sub_type_from :: "expr => nat => expr"
 where "sub_type_from (Var v) n = Var v"
@@ -292,7 +292,7 @@ where "sub_type_from (Var v) n = Var v"
     | "sub_type_from (TyLam e) n = TyLam (sub_type_from e (Suc n))"
     | "sub_type_from (TyAp t e) n = TyAp (type_sub_from n t) (sub_type_from e n)"
 
-definition safe_subst_type :: "expr => type => expr"
-where "safe_subst_type e t = sub_type_from (subst_type e (type_incr_from 0 t) 0) 0"
+definition subst_type :: "expr => type => expr"
+where "subst_type e t = sub_type_from (subst_type' e (type_incr_from 0 t) 0) 0"
 
 end
