isabelle/Chapter20_4_Abbreviations.thy
@@ -6,10 +6,10 @@ abbreviation Nat :: type
 where "Nat == Rec (Sum Unit (Tyvar 0))"
 
 lemma "is_valid_type {} Nat" by (simp add: expand_set_def)
-lemma "free_type_vars Nat = {}" by simp
+lemma "type_free_vars Nat = {}" by simp
 lemma "type_sub_from n Nat = Nat" by simp
 lemma "type_incr_from n Nat = Nat" by simp
-lemma "type_subst Nat t x = Nat" by simp
+lemma "type_subst' Nat t x = Nat" by simp
 
 abbreviation Zero :: expr
 where "Zero == Fold (Sum Unit (Tyvar 0)) (InL Unit Nat Triv)"
@@ -17,8 +17,8 @@ where "Zero == Fold (Sum Unit (Tyvar 0)) (InL Unit Nat Triv)"
 lemma "free_vars Zero = {}" by simp
 lemma "incr_from n Zero = Zero" by simp
 lemma "sub_from n Zero = Zero" by simp
-lemma "subst Zero e x = Zero" by simp
-lemma "typecheck env Zero Nat" by (simp add: safe_type_subst_def)
+lemma "subst' Zero e x = Zero" by simp
+lemma "typecheck env Zero Nat" by (simp add: type_subst_def)
 lemma "is_val Zero" by simp
 
 abbreviation Succ :: "expr => expr"
@@ -27,8 +27,8 @@ where "Succ e == Fold (Sum Unit (Tyvar 0)) (InR Unit Nat e)"
 lemma "free_vars (Succ e) = free_vars e" by simp
 lemma "incr_from n (Succ e) = Succ (incr_from n e)" by simp
 lemma "sub_from n (Succ e) = Succ (sub_from n e)" by simp
-lemma "subst (Succ n) e x = Succ (subst n e x)" by simp
-lemma "typecheck env n Nat ==> typecheck env (Succ n) Nat" by (simp add: safe_type_subst_def)
+lemma "subst' (Succ n) e x = Succ (subst' n e x)" by simp
+lemma "typecheck env n Nat ==> typecheck env (Succ n) Nat" by (simp add: type_subst_def)
 
 lemma "is_val (Succ n) = is_val n" by simp
 lemma "eval n n' ==> eval (Succ n) (Succ n')" by simp
@@ -39,39 +39,40 @@ where "IsZ et e0 e1 == Case (Unfold et) (incr_from 0 e0) e1"
 lemma "free_vars (IsZ et e0 e1) = free_vars e0 Un free_vars et Un redr_set (free_vars e1)" by auto
 lemma "incr_from n (IsZ et e0 e1) = IsZ (incr_from n et) (incr_from n e0) (incr_from (Suc n) e1)" by simp
 lemma "n ~: free_vars (IsZ et e0 e1) ==> sub_from n (IsZ et e0 e1) = IsZ (sub_from n et) (sub_from n e0) (sub_from (Suc n) e1)" by simp
-lemma "subst (IsZ et e0 e1) e x = IsZ (subst et e x) (subst e0 e x) (subst e1 (incr_from 0 e) (Suc x))" by simp
+lemma "subst' (IsZ et e0 e1) e x = IsZ (subst' et e x) (subst' e0 e x) (subst' e1 (incr_from 0 e) (Suc x))" by simp
 lemma "typecheck env et Nat ==> typecheck env e0 t ==> typecheck (extend_at env 0 Nat) e1 t ==> typecheck env (IsZ et e0 e1) t" 
 proof -
   assume "typecheck env et Nat" 
      and "typecheck env e0 t" 
      and "typecheck (extend_at env 0 Nat) e1 t"
-  moreover hence "typecheck env (Unfold et) (safe_type_subst (Sum Unit (Tyvar 0)) (Rec (Sum Unit (Tyvar 0))))" by simp
-  ultimately show "typecheck env (Case (Unfold et) (incr_from 0 e0) e1) t" by (simp add: safe_type_subst_def)
+  moreover hence "typecheck env (Unfold et) (type_subst (Sum Unit (Tyvar 0)) Nat)" by simp
+  ultimately show "typecheck env (Case (Unfold et) (incr_from 0 e0) e1) t" by (simp add: type_subst_def)
 qed
 lemma "is_val (IsZ e0 e1 e2) = False" by simp
 lemma "eval e e' ==> eval (IsZ e e0 e1) (IsZ e' e0 e1)" by simp
 lemma "EX e'. eval (IsZ Zero e0 e1) e' & eval e' e0" 
 proof -
-  have "eval (Case (InL Unit Nat Triv) (incr_from 0 e0) e1) (safe_subst (incr_from 0 e0) Triv)" by (metis ecs2 is_val.simps(5))
+  have "eval (Case (InL Unit Nat Triv) (incr_from 0 e0) e1) (subst (incr_from 0 e0) Triv)" by (metis ecs2 is_val.simps(5))
   hence "eval (Case (InL Unit Nat Triv) (incr_from 0 e0) e1) e0" by simp
-  moreover have "eval (Case (Unfold (Fold (Sum Unit (Tyvar 0)) (InL Unit Nat Triv))) (incr_from 0 e0) e1) (Case (InL Unit Nat Triv) (incr_from 0 e0) e1)" by simp
-  ultimately have "EX e'. eval (Case (Unfold (Fold (Sum Unit (Tyvar 0)) (InL Unit Nat Triv))) (incr_from 0 e0) e1) e' & eval e' e0" by fast
+  moreover have "eval (Case (Unfold Zero) (incr_from 0 e0) e1) (Case (InL Unit Nat Triv) (incr_from 0 e0) e1)" by simp
+  ultimately have "EX e'. eval (Case (Unfold Zero) (incr_from 0 e0) e1) e' & eval e' e0" by fast
   thus "EX e'. eval (IsZ Zero e0 e1) e' & eval e' e0" by simp
 qed
-lemma "is_val e ==> EX e'. eval (IsZ (Succ e) e0 e1) e' & eval e' (safe_subst e1 e)" 
+lemma "is_val e ==> EX e'. eval (IsZ (Succ e) e0 e1) e' & eval e' (subst e1 e)" 
 proof -
   assume X: "is_val e"
-  hence "eval (Case (Unfold (Fold (Sum Unit (Tyvar 0)) (InR Unit Nat e))) (incr_from 0 e0) e1) (Case (InR Unit Nat e) (incr_from 0 e0) e1)" by simp
-  moreover with X have "eval (Case (InR Unit Nat e) (incr_from 0 e0) e1) (safe_subst e1 e)" by simp
-  ultimately show "EX e'. eval (IsZ (Succ e) e0 e1) e' & eval e' (safe_subst e1 e)" by auto
+  hence "eval (Case (Unfold (Succ e)) (incr_from 0 e0) e1) (Case (InR Unit Nat e) (incr_from 0 e0) e1)" by simp
+  moreover with X have "eval (Case (InR Unit Nat e) (incr_from 0 e0) e1) (subst e1 e)" by simp
+  ultimately show "EX e'. eval (IsZ (Succ e) e0 e1) e' & eval e' (subst e1 e)" by auto
 qed
 
 lemma canonical_nat_like: "typecheck env e t ==> is_val e ==> 
     (t = Nat --> e = Zero | (EX v. typecheck env v Nat & is_val v & e = Succ v)) & 
     (t = Sum Unit Nat --> e = InL Unit Nat Triv | (EX v. typecheck env v Nat & is_val v & e = InR Unit Nat v))"
-by (induction env e t rule: typecheck.induct, auto simp add: canonical_unit safe_type_subst_def) 
+by (induction env e t rule: typecheck.induct, auto simp add: canonical_unit type_subst_def) 
 
 lemma canonical_nat: "typecheck env e Nat ==> is_val e ==> e = Zero | (EX v. typecheck env v Nat & is_val v & e = Succ v)"
 by (simp add: canonical_nat_like)
+
 
 end
